src/Examples/MapPlay.v
@@ -1,0 +1,114 @@
+Require Import Nijn.Nijn.
+Open Scope poly_scope.
+
+Inductive base_types := 
+| Ca  
+| Clist.
+
+Global Instance decEq_base_types : decEq base_types.
+Proof.
+  decEq_finite.
+Defined.
+
+
+Definition a := Base Ca.
+Definition list := Base Clist.
+
+Inductive fun_symbols := 
+| Tcons  
+| Tmap  
+| Tnil.
+
+Global Instance decEq_fun_symbols : decEq fun_symbols.
+Proof.
+  decEq_finite.
+Defined.
+
+
+Definition fn_arity fn_symbols := 
+  match fn_symbols with
+  | Tcons  =>  a ⟶ list ⟶ list
+  | Tmap  =>  list ⟶ (a ⟶ a) ⟶ list
+  | Tnil => list
+  end.
+
+Definition cons {C} : tm fn_arity C _ := BaseTm Tcons.
+Definition map {C} : tm fn_arity C _ := BaseTm Tmap.
+Definition nil {C} : tm fn_arity C _ := BaseTm Tnil.
+
+Program Definition rule_0 := 
+  make_rewrite
+    (_ ,, ∙) _
+    (map · nil ·  V 0)
+    nil.
+
+Program Definition rule_1 := 
+  make_rewrite
+    (_ ,, _ ,, _ ,, ∙) _
+    (map · (cons ·  V 0 ·  V 1) ·  V 2)
+    (cons · ( V 2 ·  V 0) · (map ·  V 1 ·  V 2)).
+
+Definition trs := 
+  make_afs
+    fn_arity 
+    (rule_0 :: rule_1 :: List.nil).
+
+Definition map_fun_poly fn_symbols : poly ∙ (arity trs fn_symbols) := 
+  match fn_symbols with
+  | Tnil => to_Poly (P_const 3)
+  | Tcons  => λP λP let y1 := P_var Vz in
+    to_Poly (P_const 3
+             + P_const 2 * y1)
+  | Tmap  =>  λP let y0 := P_var (Vs Vz) in λP let G1 := P_var Vz in
+    to_Poly (P_const 3 * y0
+             + P_const 3 * y0 * (G1 ·P (y0)))
+  end.
+
+Definition  trs_isSN : isSN trs.
+Proof.
+  solve_poly_SN map_fun_poly.
+Qed.
+
+Import AFSNotation.
+
+Locate "∼>".
+Check rew.
+
+
+Definition koe'
+  : let C := a ,, ∙ in
+    λ ((λ TmVar Vz) · TmVar Vz) ∼> λ (TmVar Vz : tm trs C _).
+Proof.
+  cbn.
+  apply rew_Lam.
+  apply rew_betaRed.
+  Print rew.
+  
+
+Definition koe
+  : let C := a ⟶ a ,, ∙ in
+    let f := TmVar (Vs (Vz)) in
+    let l := (map · nil · (λ (f · TmVar Vz))) : tm trs C list in
+    l ∼> nil.
+Proof.
+  cbn.
+  assert (In rule_0 (list_of_rewriteRules trs)) as X.
+  {
+    admit.
+  }
+  pose (MakeMem rule_0 X).
+  pose (@rew_rewrite_rule
+          _ _
+          trs
+          (MakeMem rule_0 X)
+          (a ⟶ a ,, ∙)
+          (ToEmpty _ && (λ (TmVar (Vs Vz) · TmVar Vz)))).
+  cbn in r.
+  exact r.
+  Check idSub.
+  Search sub.
+  Print members.
+  Print rewriteRules.
+  trs.
+  Search rew.
+  Print rew.
